@prefix dasb: <https://w3id.org/damagemodels/d-asb-ing#> .
@prefix owl: <http://www.w3.org/2002/07/owl#> .
@prefix foaf: <http://xmlns.com/foaf/0.1/> .
@prefix rdf: <http://www.w3.org/1999/02/22-rdf-syntax-ns#> .
@prefix xsd: <http://www.w3.org/2001/XMLSchema#> .
@prefix rdfs: <http://www.w3.org/2000/01/rdf-schema#> .
@prefix vann: <http://purl.org/vocab/vann/> .
@prefix dcterms: <http://purl.org/dc/terms/> .
@prefix dot: <https://w3id.org/dot#> .
@prefix schema: <http://schema.org/#> .
@prefix brot: <http://www.semanticweb.org/taras/ontologies/2018/7/BROT#> .
@prefix bot: <https://w3id.org/bot#> .

<https://w3id.org/damagemodels/d-asb-ing#> rdf:type owl:Ontology ;
  dcterms:creator [
      rdf:type foaf:Person ;
      foaf:name "Al-Hakam Hamdan" ;
    ] ;  
  dcterms:creator [
      rdf:type foaf:Person ;
      foaf:name "Mathias Bonduel" ;
    ] ;
	owl:versionIRI <https://w3id.org/damagemodels/d-asb-ing#/0.3.0> ;
	dcterms:description "Ontology for defining assessments of damage / defects, components and structures based on the German standard ASB-ING and DIN 1076."@en ;
	dcterms:modified "28th January 2019" ;
	dcterms:title "ASB-ING Assessment Ontology"@en ;
	dcterms:creator "Al-Hakam Hamdan" ;
	dcterms:license "https://creativecommons.org/licenses/by/1.0" ;
	vann:preferredNamespacePrefix "dasb" ;
	vann:preferredNamespaceUri "https://w3id.org/damagemodels/d-asb-ing#" .

# 
# 
# 
# #################################################################
# #
# #    Object Properties
# #
# #################################################################
# 
# 
# https://w3id.org/damagemodels/d-asb-ing#hasAssessment

dasb:hasAssessment a owl:ObjectProperty ;
	schema:domainIncludes dot:DamageElement ,
							dot:DamageArea ,
							dot:DamagePattern ,
							brot:BridgeElement ,
                            brot:BridgeSpatialZone ,
                            bot:Element ,
                            bot:Zone ;
	rdfs:range dasb:Assessment ;
	rdfs:comment "Relationship between Assessment and Damage or Structure_Element."@en ;
	rdfs:label "has Assessment"@en .
# 
# 
# 
# #################################################################
# #
# #    Data properties
# #
# #################################################################
# 
# 
# https://w3id.org/damagemodels/d-asb-ing#BWPRUFkeyword

dasb:BWPRUFkeyword a owl:DatatypeProperty ;
	rdfs:domain dot:Description ;
	rdfs:comment "Keyword for damage assessment based on the key-table of ASB-ING, Annex D (2013)."@en ;
	rdfs:label "keyword"@en .
# 
# https://w3id.org/damagemodels/d-asb-ing#assessmentFactors

dasb:assessmentFactors a owl:DatatypeProperty ;
	rdfs:domain dasb:Assessment ;
	rdfs:comment "Assessment factors, that rate the structure, component and damage / defect. Uses grades from 1-6"@en ;
	rdfs:label "assessment factors"@en .
# 
# https://w3id.org/damagemodels/d-asb-ing#durabilityFactor

dasb:durabilityFactor a owl:DatatypeProperty ;
	rdfs:subPropertyOf dasb:assessmentFactors ;
	rdfs:comment "Rating for describing the durability / influence on the durability of the structure of the assessed element (1-6)."@en ;
	rdfs:label "durabilty factor"@en .
# 
# https://w3id.org/damagemodels/d-asb-ing#overallRating

dasb:overallRating a owl:DatatypeProperty ;
	rdfs:subPropertyOf dasb:assessmentFactors ;
	rdfs:domain dasb:StructureAssessment ;
	rdfs:comment "The overall rating, that is given to the structure or sub-structure after considering the stability factor, traffic safety factor and durability factor from each assessed element. For the calculation formula see B22 of BASt[5]."@en ;
	rdfs:label "overall rating"@en .
# 
# https://w3id.org/damagemodels/d-asb-ing#stabilityFactor

dasb:stabilityFactor a owl:DatatypeProperty ;
	rdfs:subPropertyOf dasb:assessmentFactors ;
	rdfs:comment "Rating for describing the stability / influence on the stability of the structure of the assessed element (1-6)"@en ;
	rdfs:label "stability factor"@en .
# 
# https://w3id.org/damagemodels/d-asb-ing#trafficSafetyFactor

dasb:trafficSafetyFactor a owl:DatatypeProperty ;
	rdfs:subPropertyOf dasb:assessmentFactors ;
	rdfs:comment "Rating for describing the traffic safety /influence on the traffic safety of the structure of the assessed element (1-6)."@en ;
	rdfs:label "traffic safety factor"@en .
# 
# 
# 
# #################################################################
# #
# #    Classes
# #
# #################################################################
# 
# 
# https://w3id.org/damagemodels/d-asb-ing#Assessment

dasb:Assessment a owl:Class ;
	rdfs:comment "Rating for the assessed structure, following the ASB-ING standard (DIN 1076)"@en ;
	rdfs:label "Assessment"@en .
# 
# https://w3id.org/damagemodels/d-asb-ing#Component_Assessment

dasb:ComponentAssessment a owl:Class ;
	rdfs:subClassOf dasb:Assessment ;
	rdfs:comment "Assessment for a specific component."@en ;
	rdfs:label "Component Assessment"@en .
# 
# https://w3id.org/damagemodels/d-asb-ing#Damage_Assessment

dasb:DamageAssessment a owl:Class ;
	rdfs:subClassOf dasb:Assessment ;
	rdfs:comment "Assessment for a specific Damage_Element (Damage_Area or Individual_Damage)."@en ;
	rdfs:label "Damage Assessment"@en .
# 
# https://w3id.org/damagemodels/d-asb-ing#Structure_Assessment

dasb:StructureAssessment a owl:Class ;
	rdfs:subClassOf dasb:Assessment ;
	rdfs:comment "Overall assessment for the whole structure or a sub-structure (includes overall rating)."@en ;
	rdfs:label "Structure Assessment"@en .
