@prefix : <https://w3id.org/dco#> .
@prefix dce: <http://purl.org/dc/elements/1.1/> .
@prefix owl: <http://www.w3.org/2002/07/owl#> .
@prefix rdf: <http://www.w3.org/1999/02/22-rdf-syntax-ns#> .
@prefix xml: <http://www.w3.org/XML/1998/namespace> .
@prefix xsd: <http://www.w3.org/2001/XMLSchema#> .
@prefix rdfs: <http://www.w3.org/2000/01/rdf-schema#> .
@prefix vann: <http://purl.org/vocab/vann/> .
@prefix dcterms: <http://purl.org/dc/terms/> .
@base <https://w3id.org/dco#> .

<https://w3id.org/dco#> rdf:type owl:Ontology ;
                         owl:versionIRI <https://w3id.org/dco/0.1.2> ;
                         dce:Language "en" ;
                         dce:description "Ontology for damage and defects in structures." ;
                         dce:modified "October 25th 2018" ;
                         dce:title "Damage Core Ontology" ;
                         dcterms:creator "Al-Hakam Hamdan" ;
                         dcterms:description "Ontology for damage and defects in structures." ;
                         dcterms:license "https://creativecommons.org/licenses/by/1.0" ;
                         dcterms:title "Damage Core Ontology" ;
                         vann:preferredNamespacePrefix "dco" ;
                         vann:preferredNamespaceUri "https://w3id.org/dco#" .

#################################################################
#    Annotation properties
#################################################################

###  http://purl.org/dc/elements/1.1/Language
dce:Language rdf:type owl:AnnotationProperty .


###  http://purl.org/dc/elements/1.1/description
dce:description rdf:type owl:AnnotationProperty .


###  http://purl.org/dc/elements/1.1/modified
dce:modified rdf:type owl:AnnotationProperty .


###  http://purl.org/dc/elements/1.1/title
dce:title rdf:type owl:AnnotationProperty .


###  http://purl.org/dc/terms/contributor
dcterms:contributor rdf:type owl:AnnotationProperty .


###  http://purl.org/dc/terms/creator
dcterms:creator rdf:type owl:AnnotationProperty .


###  http://purl.org/dc/terms/description
dcterms:description rdf:type owl:AnnotationProperty .


###  http://purl.org/dc/terms/issued
dcterms:issued rdf:type owl:AnnotationProperty .


###  http://purl.org/dc/terms/license
dcterms:license rdf:type owl:AnnotationProperty .


###  http://purl.org/dc/terms/modified
dcterms:modified rdf:type owl:AnnotationProperty .


###  http://purl.org/dc/terms/title
dcterms:title rdf:type owl:AnnotationProperty .


###  http://purl.org/vocab/vann/preferredNamespacePrefix
vann:preferredNamespacePrefix rdf:type owl:AnnotationProperty .


###  http://purl.org/vocab/vann/preferredNamespaceUri
vann:preferredNamespaceUri rdf:type owl:AnnotationProperty .


#################################################################
#    Object Properties
#################################################################

###  https://w3id.org/dco#hasPart
:hasPart rdf:type owl:ObjectProperty ;
         rdfs:subPropertyOf <https://w3id.org/dco##contains> ;
         rdfs:domain :Component ;
         rdfs:range :Component ;
         rdfs:comment "A relationship between a component and its sub-parts (which are also components)."@en ;
         rdfs:label "has part"@en .


###  https://w3id.org/dco##combines
<https://w3id.org/dco##combines> rdf:type owl:ObjectProperty ;
                                 rdfs:subPropertyOf <https://w3id.org/dco##contains> ;
                                 rdfs:domain :Damage_Pattern ;
                                 rdfs:range :Individual_Damage ;
                                 rdfs:comment "Combines Individual Damage parts that are physically connected in a Damage Pattern."@en ;
                                 rdfs:label "combines"@en .


###  https://w3id.org/dco##consistsOf
<https://w3id.org/dco##consistsOf> rdf:type owl:ObjectProperty ;
                                   rdfs:subPropertyOf <https://w3id.org/dco##contains> ;
                                   rdfs:domain :Damage_Area ;
                                   rdfs:range :Damage_Pattern ,
                                              :Individual_Damage ;
                                   rdfs:comment "A relationship between a Damage Area and its consisting Individual Damage elements and / or Damage Patterns."@en ;
                                   rdfs:label "consists of"@en .


###  https://w3id.org/dco##contains
<https://w3id.org/dco##contains> rdf:type owl:ObjectProperty ;
                                 rdfs:domain :Damage ,
                                             :Structure_Element ;
                                 rdfs:comment "A relationship between an object and its constituent part(s)."@en ;
                                 rdfs:label "contains"@en .


###  https://w3id.org/dco##hasComponent
<https://w3id.org/dco##hasComponent> rdf:type owl:ObjectProperty ;
                                     rdfs:subPropertyOf <https://w3id.org/dco##contains> ;
                                     rdfs:domain :Structure ;
                                     rdfs:range :Component ;
                                     rdfs:comment "The relationship between a structure and its component."@en ;
                                     rdfs:label "has component"@en .


###  https://w3id.org/dco##hasDamage
<https://w3id.org/dco##hasDamage> rdf:type owl:ObjectProperty ;
                                  rdfs:subPropertyOf <https://w3id.org/dco##contains> ;
                                  rdfs:domain :Component ;
                                  rdfs:range :Damage_Area ;
                                  rdfs:comment "The relationship between a Component and its belonging Damage Area."@en ;
                                  rdfs:label "has damage"@en .


###  https://w3id.org/dco##hasDocumentation
<https://w3id.org/dco##hasDocumentation> rdf:type owl:ObjectProperty ;
                                         rdfs:subPropertyOf owl:topObjectProperty ;
                                         rdfs:domain :Damage ,
                                                     :Structure_Element ;
                                         rdfs:range :Documentation ;
                                         rdfs:comment "Relationship between a Documenation and the relevant documented or inspected object which could be either a Damage or a Structure Element."@en ;
                                         rdfs:label "has Documentation"@en .


#################################################################
#    Data properties
#################################################################

###  https://w3id.org/dco#content
:content rdf:type owl:DatatypeProperty ;
         rdfs:domain :Description ;
         rdfs:comment "Textual content used for the Description of a Structure Element or Damage."@en ;
         rdfs:label "content"@en .


###  https://w3id.org/dco##author
<https://w3id.org/dco##author> rdf:type owl:DatatypeProperty ;
                               rdfs:subPropertyOf <https://w3id.org/dco##metadata> ;
                               rdfs:comment "Name of the responsible person or company that created the record of the related element."@en ;
                               rdfs:label "author"@en .


###  https://w3id.org/dco##creationDate
<https://w3id.org/dco##creationDate> rdf:type owl:DatatypeProperty ;
                                     rdfs:subPropertyOf <https://w3id.org/dco##metadata> ;
                                     rdfs:comment "Date and time in which the relevant element has been firstly created by the author."@en ;
                                     rdfs:label "creation date"@en .


###  https://w3id.org/dco##lastModification
<https://w3id.org/dco##lastModification> rdf:type owl:DatatypeProperty ;
                                         rdfs:subPropertyOf <https://w3id.org/dco##metadata> ;
                                         rdfs:comment "Date and time of the last modification for the relevant element."@en ;
                                         rdfs:label "last modification"@en .


###  https://w3id.org/dco##metadata
<https://w3id.org/dco##metadata> rdf:type owl:DatatypeProperty ;
                                 rdfs:domain :Damage ,
                                             :Documentation ,
                                             :Structure_Element .


###  https://w3id.org/dco##name
<https://w3id.org/dco##name> rdf:type owl:DatatypeProperty ;
                             rdfs:subPropertyOf <https://w3id.org/dco##metadata> ;
                             rdfs:comment "A given name for the relevant element by the author. Optional and only used for easier identification by humans besides the IRI."@en ;
                             rdfs:label "name"@en .


###  https://w3id.org/dco##version
<https://w3id.org/dco##version> rdf:type owl:DatatypeProperty ;
                                rdfs:subPropertyOf <https://w3id.org/dco##metadata> ;
                                rdfs:comment "Version number of the relevant element. Should be changed after every modficiation of the element."@en ;
                                rdfs:label "version"@en .


#################################################################
#    Classes
#################################################################

###  https://w3id.org/dco#Component
:Component rdf:type owl:Class ;
           rdfs:subClassOf :Structure_Element ;
           owl:disjointWith :Structure ;
           rdfs:comment "Object that is part of a structure."@en ;
           rdfs:label "Component"@en .


###  https://w3id.org/dco#Damage
:Damage rdf:type owl:Class ;
        owl:disjointWith :Documentation ,
                         :Structure_Element ;
        owl:disjointUnionOf ( :Damage_Area
                              :Damage_Pattern
                              :Individual_Damage
                            ) ,
                            ( :Defect
                              :Structural_Damage
                            ) ;
        rdfs:comment "Damage is the harm to a structure resulting in impairment or loss of function, usefulness or value."@en ;
        rdfs:label "Damage"@en .


###  https://w3id.org/dco#Damage_Area
:Damage_Area rdf:type owl:Class ;
             rdfs:subClassOf :Damage ;
             owl:disjointWith :Damage_Pattern ,
                              :Individual_Damage ;
             rdfs:comment "Area in a component where damage is located."@en ;
             rdfs:label "Damage Area"@en .


###  https://w3id.org/dco#Damage_Pattern
:Damage_Pattern rdf:type owl:Class ;
                rdfs:subClassOf :Damage ;
                owl:disjointWith :Individual_Damage ;
                rdfs:comment "Defines a group of physically connected individual damage elements."@en ;
                rdfs:label "Damage Pattern"@en .


###  https://w3id.org/dco#Defect
:Defect rdf:type owl:Class ;
        rdfs:subClassOf :Damage ;
        owl:disjointWith :Structural_Damage ;
        rdfs:comment "Damage that does not impair the structural integrity of the structure, but can still have influence on the durability, usability and / or value."@en ;
        rdfs:label "Defect"@en .


###  https://w3id.org/dco#Description
:Description rdf:type owl:Class ;
             rdfs:subClassOf :Documentation ;
             owl:disjointWith :External_Ressource ;
             rdfs:comment "Short textual documentation about a Damage or Structure Element. Generally created by the inspecting person."@en ;
             rdfs:label "Description"@en .


###  https://w3id.org/dco#Documentation
:Documentation rdf:type owl:Class ;
               owl:disjointWith :Structure_Element ;
               owl:disjointUnionOf ( :Description
                                     :External_Ressource
                                   ) ;
               rdfs:comment "Material or data that provides information or evidence about the structure and its components or that serves as a record."@en ;
               rdfs:label "Documentation"@en .


###  https://w3id.org/dco#External_Ressource
:External_Ressource rdf:type owl:Class ;
                    rdfs:subClassOf :Documentation ;
                    rdfs:comment "Document that is stored in a separate file, referenced by an external path."@en ;
                    rdfs:label "External Ressource"@en .


###  https://w3id.org/dco#Individual_Damage
:Individual_Damage rdf:type owl:Class ;
                   rdfs:subClassOf :Damage ;
                   rdfs:comment "Damage that is modelled on a very detailled level and belongs with other adjacent individual damage elements to a broader damage area."@en ;
                   rdfs:label "Individual Damage"@en .


###  https://w3id.org/dco#Structural_Damage
:Structural_Damage rdf:type owl:Class ;
                   rdfs:subClassOf :Damage ;
                   rdfs:comment "Damage that impairs the structural integrity of the structure."@en ;
                   rdfs:label "Structural Damage"@en .


###  https://w3id.org/dco#Structure
:Structure rdf:type owl:Class ;
           rdfs:subClassOf :Structure_Element ;
           rdfs:comment "Something (such as a building or a bridge) that is constructed."@en ;
           rdfs:label "Structure"@en .


###  https://w3id.org/dco#Structure_Element
:Structure_Element rdf:type owl:Class ;
                   owl:disjointUnionOf ( :Component
                                         :Structure
                                       ) ;
                   rdfs:comment "Objects that are damaged."@en ;
                   rdfs:label "Structure Element"@en .


###  Generated by the OWL API (version 4.5.6.2018-09-06T00:27:41Z) https://github.com/owlcs/owlapi
