@prefix dot: <https://w3id.org/dot#> .
@prefix bot: <https://w3id.org/bot#> .
@prefix owl: <http://www.w3.org/2002/07/owl#> .
@prefix rdf: <http://www.w3.org/1999/02/22-rdf-syntax-ns#> .
@prefix xsd: <http://www.w3.org/2001/XMLSchema#> .
@prefix brot: <https://wisib.de/ontologie/brot#> .
@prefix foaf: <http://xmlns.com/foaf/0.1/> .
@prefix rdfs: <http://www.w3.org/2000/01/rdf-schema#> .
@prefix voaf: <http://purl.org/vocommons/voaf#> .
@prefix vann: <http://purl.org/vocab/vann/> .
@prefix schema: <http://schema.org/#> .
@prefix dcterms: <http://purl.org/dc/terms/> .

<https://w3id.org/dot#> rdf:type owl:Ontology , voaf:Vocabulary ;
	dcterms:creator [
      rdf:type foaf:Person ;
      foaf:name "Al-Hakam Hamdan" ;
    ] ;  
	dcterms:creator <https://www.researchgate.net/profile/Mathias_Bonduel> ;
	owl:versionIRI <https://w3id.org/dot/0.8> ;
	owl:versionInfo "0.8" ;
	rdfs:comment """- Version 0.8: 
* completed ontology metadata wrt LOV
* added classes dot:ClassifiedDamage and dot:UnclassifiedDamage (subclasses of dot:Damage)
* made dot:StructuralDamage and dot:Defect subclasses of dot:Damage
"""@en ;
	dcterms:description "Ontology that defines the topology of damages in constructions."@en ;
	dcterms:license "https://creativecommons.org/licenses/by/1.0" ;
	dcterms:modified "2019-12-17"^^xsd:date ;
	dcterms:issued "2018-10-12"^^xsd:date ;
	dcterms:title "Damage Topology Ontology"@en ;
	vann:example "https://madsholten.github.io/sparql-visualizer/?file=https://raw.githubusercontent.com/Alhakam/dot/master/ABox-Examples/dot-demo.json"^^xsd:anyURI ;
	vann:example "https://raw.githubusercontent.com/Alhakam/dot/master/ABox-Examples/dotSampleData_pt1.ttl"^^xsd:anyURI ;
	vann:example "https://raw.githubusercontent.com/Alhakam/dot/master/ABox-Examples/dotSampleData_pt2.ttl"^^xsd:anyURI ;
	vann:preferredNamespacePrefix "dot" ;
	vann:preferredNamespaceUri "https://w3id.org/dot#" .

#################################################################
#    Object Properties
#################################################################

###  https://w3id.org/dot#adjacentDamageElement
dot:adjacentDamageElement rdf:type owl:ObjectProperty ,
                                   owl:SymmetricProperty ;
                          rdfs:domain dot:DamageElement ;
                          rdfs:range dot:DamageElement ;
                          rdfs:comment "Defines the relationship between two instances of Damage Element that are physically connected with each other."@en ;
						  rdfs:isDefinedBy dot: ;
                          rdfs:label "adjacent Damage Element"@en .


###  https://w3id.org/dot#aggregatesDamageElement
dot:aggregatesDamageElement rdf:type owl:ObjectProperty ;
                            rdfs:domain dot:DamageArea ;
                            rdfs:range dot:DamageElement ;
                            owl:propertyChainAxiom ( dot:aggregatesDamageElement
                                                     dot:adjacentDamageElement
                                                   ) ,
                                                   ( dot:aggregatesDamagePattern
                                                     dot:groupsDamageElement
                                                   ) ;
                            rdfs:comment "A relationship between an instance of Damage Area and its consisting DamageElement instance."@en ;
							rdfs:isDefinedBy dot: ;
                            rdfs:label "aggregates Damage Element"@en .


###  https://w3id.org/dot#aggregatesDamagePattern
dot:aggregatesDamagePattern rdf:type owl:ObjectProperty ;
                            rdfs:domain dot:DamageArea ;
                            rdfs:range dot:DamagePattern ;
                            rdfs:comment "A relationship between an instance of Damage Area and its consisting Damage Pattern instance."@en ;
							rdfs:isDefinedBy dot: ;
                            rdfs:label "aggregates Damage Pattern"@en .


###  https://w3id.org/dot#groupsDamageElement
dot:groupsDamageElement rdf:type owl:ObjectProperty ;
                        rdfs:domain dot:DamagePattern ;
                        rdfs:range dot:DamageElement ;
                        owl:propertyChainAxiom ( dot:groupsDamageElement
                                                 dot:adjacentDamageElement
                                               ) ;
                        rdfs:comment "Groups instances of Damage Element that are physically connected in a Damage Pattern."@en ;
						rdfs:isDefinedBy dot: ;
                        rdfs:label "groups Damage Element"@en .


###  https://w3id.org/dot#hasCausation
dot:hasCausation rdf:type owl:ObjectProperty ;
                 rdfs:domain dot:Damage ;
                 rdfs:range dot:Causation ;
                 rdfs:comment "Relationship between a Damage and its Causation."@en ;
				 rdfs:isDefinedBy dot: ;
                 rdfs:label "has Causation"@en .


###  https://w3id.org/dot#hasDamage
dot:hasDamage rdf:type owl:ObjectProperty ;
              rdfs:range dot:Damage ;
              schema:domainIncludes brot:BridgeElement ,
                                    brot:BridgeSpatialZone ,
                                    bot:Element ,
                                    bot:Zone ;
              rdfs:comment "Defines the relationship between an affected component or structure (e.g. bot:Element) and a Damage."@en ;
			  rdfs:isDefinedBy dot: ;
              rdfs:label "has Damage"@en .


###  https://w3id.org/dot#hasDamageArea
dot:hasDamageArea rdf:type owl:ObjectProperty ;
                  rdfs:subPropertyOf dot:hasDamage ;
                  rdfs:range dot:DamageArea ;
                  rdfs:comment "Defines the relationship between an affected component or structure (e.g. bot:Element) and a Damage Area."@en ;
				  rdfs:isDefinedBy dot: ;
                  rdfs:label "has Damage Area"@en .


###  https://w3id.org/dot#hasDamageElement
dot:hasDamageElement rdf:type owl:ObjectProperty ;
                     rdfs:subPropertyOf dot:hasDamage ;
                     rdfs:range dot:DamageElement ;
                     owl:propertyChainAxiom ( dot:hasDamageArea
                                              dot:aggregatesDamageElement
                                            ) ;
                     rdfs:comment "Defines the relationship between an affected component or structure (e.g. bot:Element) and a Damage Element."@en ;
					 rdfs:isDefinedBy dot: ;
                     rdfs:label "has Damage Element"@en .


###  https://w3id.org/dot#coveredInDocumentation
dot:coveredInDocumentation rdf:type owl:ObjectProperty ;
                     rdfs:range dot:Documentation ;
                     schema:domainIncludes brot:BridgeElement ,
                                           brot:BridgeSpatialZone ,
                                           bot:Element ,
                                           bot:Zone ,
                                           dot:Damage ;
                     rdfs:comment "Relationship between a Documentation and the relevant documented or inspected object (e.g. DamageArea or bot:Element). Should only be used for damage-relevant documentations."@en ;
					 rdfs:isDefinedBy dot: ;
                     rdfs:label "covered by documentation"@en .


###  https://w3id.org/dot#hasInspector
dot:hasInspector rdf:type owl:ObjectProperty ;
                 rdfs:domain dot:Inspection ;
                 rdfs:range dot:Inspector ;
                 rdfs:comment "Relationship between an Inspector and the Inspection that has been performed by him."@en ;
				 rdfs:isDefinedBy dot: ;
                 rdfs:label "has Inspector"@en .


###  https://w3id.org/dot#coveredByInspection
dot:coveredByInspection rdf:type owl:ObjectProperty ;
                        schema:domainIncludes dot:Damage ,
                                              brot:BridgeElement ,
                                              brot:BridgeSpatialZone ,
                                              bot:Element ,
                                              bot:Zone ;
                        rdfs:range dot:Inspection ;
                        owl:propertyChainAxiom ( dot:coveredInDocumentation
                                                 dot:documentationFromInspection
                                               ) ;
                        rdfs:comment "Relationship between a documented object (damage or component / zone) and the Inspection in which the object has been covered."@en ;
                        rdfs:isDefinedBy dot: ;
						rdfs:label "covered by inspection"@en .


###  https://w3id.org/dot#hasDocumentation
dot:hasDocumentation rdf:type owl:ObjectProperty ;
                     owl:inverseOf dot:documentationFromInspection ;
                     rdfs:domain dot:Inspection ;
                     rdfs:range dot:Documentation ;
                     rdfs:comment "Relationship between an Inspection and the corresponding Documentation"@en ;
					 rdfs:isDefinedBy dot: ;
                     rdfs:label "has Documentation"@en .


###  https://w3id.org/dot#documentationFromInspection
dot:documentationFromInspection rdf:type owl:ObjectProperty ;
                                owl:inverseOf dot:hasDocumentation ;
                                rdfs:comment "Relationship between a Documentation and the Inspection to which the Documentation refers. Inverse object property of dot:hasDocumentation ."@en ;
                                rdfs:isDefinedBy dot: ;
								rdfs:label "documentation from inspection"@en .

#################################################################
#    Data properties
#################################################################

###  https://w3id.org/dot#filePath
dot:filePath rdf:type owl:DatatypeProperty ;
             rdfs:domain dot:ExternalResource ;
             rdfs:range xsd:anyURI ;
             rdfs:comment "Defines the unique location in a file system of an ExternalResource"@en ;
             rdfs:isDefinedBy dot: ;
			 rdfs:label "file path"@en .

###  https://w3id.org/dot#descriptionContent
dot:descriptionContent rdf:type owl:DatatypeProperty ;
                       rdfs:comment "Textual content used for the Description of a Structure Element or Damage."@en ;
                       rdfs:label "description content"@en ;
                       rdfs:subPropertyOf dcterms:description ;
                       rdfs:isDefinedBy dot: ;
					   rdfs:range xsd:string ;
                       rdfs:domain dot:Description .


#################################################################
#    Classes
#################################################################

###  https://w3id.org/dot#Causation
dot:Causation rdf:type owl:Class ;
              rdfs:comment """Represents the causation of a damage. 
Should be extended with domain-specific subclasses."""@en ;
			  rdfs:isDefinedBy dot: ;
              rdfs:label "Causation"@en .


###  https://w3id.org/dot#ClassifiedDamage
dot:ClassifiedDamage rdf:type owl:Class ;
			  rdfs:subClassOf dot:Damage ;
			  owl:disjointWith dot:UnclassifiedDamage ;
              rdfs:comment """A damage classification is used to denote the kind of damage. Subclasses of this class are defined in extensions 
			  such as CDO (Concrete Damage Ontology), NSO (the Natural Stone Ontology), etc."""@en ;
			  rdfs:isDefinedBy dot: ;
              rdfs:label "Classified Damage"@en .

###  https://w3id.org/dot#Damage
dot:Damage rdf:type owl:Class ;
           rdfs:comment """Damage is the harm to a structure resulting in impairment or loss of function, usefulness or value.
Instead of using dot:Damage, it is recommended to use one subclass of dot:Damage for respectively the damage topology (either dot:DamageArea or dot:DamageElement), the 
potential structural impact (either dot:StructuralDamage or dot:Defect) and the damage classification (either dot:UnclassifiedDamage or subclasses of dot:ClassifiedDamage)."""@en ;
           rdfs:isDefinedBy dot: ;
		   rdfs:label "Damage"@en .


###  https://w3id.org/dot#DamageArea
dot:DamageArea rdf:type owl:Class ;
               rdfs:subClassOf dot:Damage ;
               owl:disjointWith dot:DamageElement ,
                                dot:DamagePattern ;
               rdfs:comment "Area in a component where damage is located. Holds collection of multiple DamageElements or DamagePatterns. Used to be attached with simplified geometry."@en ;
               rdfs:isDefinedBy dot: ;
			   rdfs:label "Damage Area"@en .


###  https://w3id.org/dot#DamageElement
dot:DamageElement rdf:type owl:Class ;
                  rdfs:subClassOf dot:Damage ;
                  owl:disjointWith dot:DamagePattern ;
                  rdfs:comment "Damage that is modeled on a very detailed level and belongs with other adjacent Damage Element instances to a broader damage area or damage pattern"@en ;
                  rdfs:isDefinedBy dot: ;
				  rdfs:label "Damage Element"@en .


###  https://w3id.org/dot#DamagePattern
dot:DamagePattern rdf:type owl:Class ;
                  rdfs:comment "Defines a group of associated or physically connected instances of DamageElement. Used as class for grouping inside an instance of DamageArea."@en ;
                  rdfs:isDefinedBy dot: ;
				  rdfs:label "Damage Pattern"@en .


###  https://w3id.org/dot#Defect
dot:Defect rdf:type owl:Class ;
		   rdfs:subClassOf dot:Damage ;
           owl:disjointWith dot:StructuralDamage ;
           rdfs:comment """Should be used on nodes that are already classified as dot:DamageArea or dot:DamageElement.
Damage that does not impair the structural integrity of the structure, but can still have influence on the durability, usability and / or value."""@en ;
           rdfs:isDefinedBy dot: ;
		   rdfs:label "Defect"@en .


###  https://w3id.org/dot#Description
dot:Description rdf:type owl:Class ;
                rdfs:subClassOf dot:Documentation ;
                rdfs:comment "Short textual documentation about a Damage or Structure Element. Generally created by the inspecting person."@en ;
                rdfs:isDefinedBy dot: ;
				rdfs:label "Description"@en .


###  https://w3id.org/dot#Documentation
dot:Documentation rdf:type owl:Class ;
                  rdfs:comment "Material or data that provides information or evidence about the structure and its components or that serves as a record. Should only be used for damage-related documentation."@en ;
                  rdfs:isDefinedBy dot: ;
				  rdfs:label "Damage Documentation"@en .


###  https://w3id.org/dot#ExternalResource
dot:ExternalResource rdf:type owl:Class ;
                     rdfs:subClassOf dot:Documentation ;
                     rdfs:comment "Document that is stored in a separate file, referenced by an external path."@en ;
                     rdfs:isDefinedBy dot: ;
					 rdfs:label "External Resource"@en .


###  https://w3id.org/dot#Inspection
dot:Inspection rdf:type owl:Class ;
               rdfs:comment """Careful examination or scrutiny in which an existing construction or a part of it is inspected and detected damages are recorded.
Should be repeated at regular time intervals."""@en ;
               rdfs:isDefinedBy dot: ;
			   rdfs:label "Inspection"@en .


###  https://w3id.org/dot#Inspector
dot:Inspector rdf:type owl:Class ;
              rdfs:subClassOf foaf:Person ;
              rdfs:comment "A person who inspects constructions (for damages) or whose task it is to carry out inspections on constructions."@en ;
              rdfs:isDefinedBy dot: ;
			  rdfs:label "Inspector"@en .


###  https://w3id.org/dot#StructuralDamage
dot:StructuralDamage rdf:type owl:Class ;
					 rdfs:subClassOf dot:Damage ;
                     rdfs:comment """Should be used on nodes that are already classified as dot:DamageArea or dot:DamageElement.
Damage that impairs the structural integrity of the structure."""@en ;
                     rdfs:isDefinedBy dot: ;
					 rdfs:label "Structural Damage"@en .


###  https://w3id.org/dot#UnclassifiedDamage
dot:UnclassifiedDamage rdf:type owl:Class ;
					   rdfs:subClassOf dot:Damage ;
                       rdfs:comment """A dot:Damage instance that is not further classified with domain-specific classes (subclasses of dot:ClassifiedDamage). 
This class can be used in cases where the damage classification is unknown."""@en ;
                       rdfs:isDefinedBy dot: ;
					   rdfs:label "Unclassified Damage"@en .